Veritas.Verifier.TSLog.fsti
@@ -135,12 +135,6 @@ val lemma_verifier_thread_state_extend (itsl: its_log) (i: I.seq_index itsl):
   Lemma (thread_state_post itsl i == 
          t_verify_step (thread_state_pre itsl i) (I.index itsl i))
 
-(* If the i'th entry does not go to thread tid, then its state remains unchanged when processing 
- * the i'th entry *)
-val lemma_verifier_thread_state_extend2 (itsl: its_log) (i: I.seq_index itsl) (tid: valid_tid itsl):
-  Lemma (requires (tid <> thread_id_of itsl i))
-        (ensures (thread_state (I.prefix itsl (i + 1)) tid == 
-                  thread_state (I.prefix itsl i) tid))
 
 (* is this an evict add consistent log *)
 val is_eac (itsl: its_log):bool
@@ -254,6 +248,13 @@ let lemma_verifier_boundary_thread_state (itsl: neac_log):
                                 (I.index itsl (eac_boundary itsl))))
         [SMTPat (eac_boundary itsl)] =
   lemma_verifier_thread_state_extend itsl (eac_boundary itsl)
+
+(* If the i'th entry does not go to thread tid, then its state remains unchanged when processing 
+ * the i'th entry *)
+val lemma_verifier_thread_state_extend2 (itsl: its_log) (i: I.seq_index itsl) (tid: valid_tid itsl):
+  Lemma (requires (tid <> thread_id_of itsl i))
+        (ensures (thread_state (I.prefix itsl (i + 1)) tid == 
+                  thread_state (I.prefix itsl i) tid))
 
 (* when the eac state of a key is "instore" then there is always a previous add *)
 val lemma_eac_state_active_implies_prev_add (itsl: eac_log) 
